theories/c_interface/notation.v
@@ -6,6 +6,12 @@ Coercion LitInt : Z >-> base_lit.
 Coercion LitBool : bool >-> base_lit.
 Coercion LitLoc : loc >-> base_lit.
 
-(* No scope, does not conflict and scope is often not inferred properly. *)
+(* # has no scope for historical reasons, but does conflict with the same
+   notation on the ML side. Unfortunately, guessing the scope using type
+   information is often insufficient because type inference does not flow in the
+   direction we would want. So we keep this global for now, and use #C whenever
+   we need to be explicit. *)
 Notation "# l" := (LitV l%Z%CV%stdpp) (at level 8, format "# l").
+Notation "#C l" := (LitV l%Z%CV%stdpp) (at level 8, format "#C l").
+
 Notation "& f" := (LitV (LitFunPtr f)) (at level 8, format "& f").
